
\begin{sol}{prob01.1} Express the following complex numbers in  Cartesian form: $a + b \,i$, with $a, b \in \R$.
\medskip
\begin{enumerate}[a)]
\item    $(2+i)(2+2 i)=2+6i$ \medskip  
\item $ \dfrac 1{1+i}=\dfrac{1}{2}- \dfrac{1}{2} i$\medskip 
\item $  \dfrac{8+3i}{5-3i}=\dfrac{31}{34}-\dfrac{39}{34}i$\medskip 
\item $\dfrac{5+5 \,i}{1-i}= 5 i$\medskip
% 
\item $\dfrac{(1+2i)(2+5i)}{3+4i}=\dfrac{ 12}{25} +\dfrac{59}{25}i  $

\item $\dfrac{1-i}{2-i}+\dfrac{2+i}{1-i}= \dfrac{11}{10}+\dfrac{13 }{10}i$\smallskip
% 
\item $\dfrac 1{(1-i)(3-2i)}=\dfrac{1}{26}+\dfrac{5 }{26}i$
%
\end{enumerate}

\end{sol} 

\begin{sol}{prob01.2} Find the polar form of the following complex numbers: (i.e. either  as $r e^{i\theta}$ or as $r(\cos \theta + i \sin \theta)$, with $r\geq 0$ and $-\pi <\theta \leq \pi$)\medskip
\begin{enumerate}[a)]

\item ${3\sqrt{3}-3i}=6(\cos (-\pi /6)+i \sin (-\pi /6))=6\, e^{-\frac{\pi}{6}i} $
\item $\dfrac{3\sqrt{3}-3i} {\sqrt{2}+i\sqrt{2}}=3(\cos (-5\pi /12)+i \sin (-5\pi /12)) =3\, e^{-\frac{5\pi}{12}i} $

\item $\dfrac{1-\sqrt{3}\,i}{-1+i}=\sqrt{2}(\cos (11\pi/12)+i\sin (11\pi /12))=\sqrt{2}\, e^{\frac{11\pi}{12}i} $
\item $\dfrac{5+5\sqrt{3}\,i}{\sqrt{2}-\sqrt{2}\,i}=5(\cos (7\pi /12)+i\sin (7\pi/12))= 5\,e^{\frac{7\pi}{12}i}$
\item $\dfrac{3+3\sqrt{3}\,i} {-2+2i}=\dfrac{3\sqrt{2}}{2}(\cos (5\pi /12)-i\sin (5\pi/12))=\dfrac{3\sqrt{2}}{2}\,e^{\frac{5\pi}{12}i}$
\end{enumerate}

\end{sol} 


 

\begin{sol}{prob01.4}   If $z$ is a complex number,

(i)  Is it possible that $z={\bar z}$? \soln (Yes, iff $z\in \R$:if $z=a + b\, i$, then $z={\bar z}$ iff $a + b\, i = a - b\, i )$ iff $b=-b$ iff $z=a \in \R$.

(ii)  Is it possible that $|{\bar z}|>|z|$? \soln (No: $|{\bar z}|=|z|$, always: if $z=a + b\, i$, then $|z|=\sqrt{a^2+b^2}=\sqrt{a^2+(-b)^2} =|{\bar z}|$.)

(iii)  Is it possible that ${\bar z}=2z$? \soln(Yes, but only if $z=0$: If ${\bar z}=2z$, then by the previous part, $|z|=2 |z|$, so $|z|=0$. So $z=0$ too.)

\medskip Give  examples to illustrate your affirmative answers, and explanations if you say the statement is always false.
\end{sol}